Write specs for block allocator

src/program_proof/simplefs/alloc_proof.v
@@ -1,9 +1,127 @@
 From Perennial.program_proof Require Import proof_prelude.
+From Perennial.program_proof Require Import disk_prelude.
+
 From Goose.github_com Require Import tchajed.simplefs.alloc.
 
-From Perennial.program_proof Require Import disk_prelude.
 From Perennial.goose_lang.lib Require Import typed_slice.
 
 From Perennial.program_proof.simplefs Require Import
+  superblock_proof
   inode_proof
   bitmap_proof.
+
+From Perennial Require Import options.
+
+Section proof.
+Context `{!heapGS Σ}.
+Context `{!superblockG Σ}.
+
+Definition free_block γsb_var (a: w32): iProp _ :=
+  ∃ sb,
+  "#Hsb" ∷ is_sb γsb_var sb ∗
+  "%Hbound" ∷ ⌜0 < uint.Z a < uint.Z sb.(data_blocks)⌝ ∗
+  "Hdisk_ptsto" ∷ ∃ b, (uint.Z a + sb_data_start sb) d↦ b.
+
+Lemma free_block_conflict γ a :
+  free_block γ a -∗ free_block γ a -∗ ⌜False⌝.
+Proof.
+  iIntros "H1 H2".
+  iDestruct "H1" as (sb) "(#Hsb1 & _ & (%b1 & H1))".
+  iDestruct "H2" as (sb') "(#Hsb2 & _ & (%b2 & H2))".
+  rewrite /named.
+  iDestruct (is_sb_agree with "Hsb1 Hsb2") as %<-.
+  iDestruct (gen_heap.pointsto_ne with "H1 H2") as %Hne.
+  congruence.
+Qed.
+
+Definition own_block_alloc γsb_var (l: loc): iProp _ :=
+  ∃ (offset: w64) (bm_v: val) (free_s: Slice.t),
+  "offset" ∷ l ↦[BlockAllocator :: "offset"] #offset ∗
+  "bitmap" ∷ l ↦[BlockAllocator :: "bitmap"] bm_v ∗
+  "free" ∷ l ↦[BlockAllocator :: "free"] free_s ∗
+  "d" ∷ l ↦[BlockAllocator :: "d"] #() ∗
+  ∃ (bits: list bool) (bit_data: list Block) (sb: superblockT) (free: list w32),
+  "Hbitmap" ∷ own_bitmap bm_v bits ∗
+  "%Hbit_len" ∷ ⌜length bits = uint.nat sb.(data_bitmap_blocks)⌝ ∗
+  "#Hoffset" ∷ is_sb γsb_var sb ∗
+               ⌜uint.Z offset = sb_data_bitmap_start sb⌝ ∗
+  (* this invariant will require that the on-disk bitmap reflects the
+  in-memory one *)
+  "Hdisk_bs" ∷ uint.Z offset d↦∗ bit_data ∗
+  "%Hbit_data_len" ∷ ⌜blocks_to_bits bit_data = bits⌝ ∗
+  "Hfree_list" ∷ own_slice free_s uint32T (DfracOwn 1) free ∗
+  "Hfree_bs" ∷ [∗ list] a ∈ free,
+    ⌜bits !! uint.nat a = Some false⌝ ∗
+    free_block γsb_var a
+  .
+
+(* note we're only proving this theorem starting from a zero'd bitmap
+region; a more complicated spec is needed to describe a correctly encoded
+on-disk bitmap that we then load *)
+Theorem wp_NewBlockAllocator γsb_var (sb_l : loc) sb :
+  {{{ is_superblock γsb_var sb_l sb ∗
+        (* zero'd bitmap *)
+      sb_data_bitmap_start sb d↦∗ (replicate (uint.nat sb.(data_bitmap_blocks)) block0) ∗
+        (* arbitrary data blocks *)
+      (∃ data, sb_data_start sb d↦∗ data ∗ ⌜length data = uint.nat sb.(data_blocks)⌝)
+  }}}
+    NewBlockAllocator #() #sb_l
+  {{{ (l : loc), RET #l; own_block_alloc γsb_var l }}}.
+Proof.
+  (*@ func NewBlockAllocator(d disk.Disk, sb *superblock.Superblock) *BlockAllocator { @*)
+  (*@     offset := sb.DataBitmapStart()                                      @*)
+  (*@     bm := bitmap.NewBitmapFromBlocks(d, sb.DataBitmapStart(), sb.DataBitmapBlocks) @*)
+  (*@     var free = []uint32{}                                               @*)
+  (*@     // skip 0 intentionally                                             @*)
+  (*@     for i := uint32(1); i < uint32(sb.DataBlocks); i++ {                @*)
+  (*@         if !bm.Get(uint64(i)) {                                         @*)
+  (*@             free = append(free, i)                                      @*)
+  (*@         }                                                               @*)
+  (*@     }                                                                   @*)
+  (*@     return &BlockAllocator{                                             @*)
+  (*@         offset: offset,                                                 @*)
+  (*@         bitmap: bm,                                                     @*)
+  (*@         free:   free,                                                   @*)
+  (*@         d:      d,                                                      @*)
+  (*@     }                                                                   @*)
+  (*@ }                                                                       @*)
+Admitted.
+
+Theorem wp_BlockAllocator__Alloc γ (ba : loc) :
+  {{{ own_block_alloc γ ba }}}
+    BlockAllocator__Alloc #ba
+  {{{ (a : u32) (ok : bool), RET (#a, #ok);
+      own_block_alloc γ ba ∗
+      (⌜ok = true⌝ -∗ free_block γ a)
+  }}}.
+Proof.
+  (*@ func (ba *BlockAllocator) Alloc() (uint32, bool) {                      @*)
+  (*@     if len(ba.free) == 0 {                                              @*)
+  (*@         return 0, false                                                 @*)
+  (*@     }                                                                   @*)
+  (*@     i := ba.free[len(ba.free)-1]                                        @*)
+  (*@     ba.free = ba.free[:len(ba.free)-1]                                  @*)
+  (*@     ba.bitmap.Set(uint64(i))                                            @*)
+  (*@     ba.bitmap.Write(ba.d, ba.offset)                                    @*)
+  (*@     return i, true                                                      @*)
+  (*@ }                                                                       @*)
+Admitted.
+
+Theorem wp_BlockAllocator__Free γ (ba : loc) (a : u32) :
+  {{{ own_block_alloc γ ba ∗
+      free_block γ a
+  }}}
+    BlockAllocator__Free #ba #a
+  {{{ RET #(); own_block_alloc γ ba }}}.
+Proof.
+  (*@ func (ba *BlockAllocator) Free(i uint32) {                              @*)
+  (*@     if !ba.bitmap.Get(uint64(i)) {                                      @*)
+  (*@         panic("freeing free block")                                     @*)
+  (*@     }                                                                   @*)
+  (*@     ba.bitmap.Clear(uint64(i))                                          @*)
+  (*@     ba.bitmap.Write(ba.d, ba.offset)                                    @*)
+  (*@     ba.free = append(ba.free, i)                                        @*)
+  (*@ }                                                                       @*)
+Admitted.
+
+End proof.
